Problems/SetCover.dfy
@@ -1,5 +1,4 @@
 
-  
 ghost predicate isCover<T>(universe:set<T>, sets:set<set<T>>)
 {
   forall e | e in universe :: (exists s | s in sets :: e in s)
